src/Noninterference/LoggedDisk/TS/ATCD_TS_BatchOperations.v
@@ -1,0 +1,203 @@
+Require Import Eqdep Lia Framework FSParameters CryptoDiskLayer BatchOperations.
+
+Set Nested Proofs Allowed.
+
+  
+  Lemma BatchOperations_TS_hash_all:
+  forall u l1 l2 s1 s2 o s1' t h1 h2,
+  exec (CryptoDiskLang) u o s1 
+  (hash_all h1 l1)
+       (Finished s1' t) ->
+  length l1 = length l2 ->
+  consistent_with_upds (snd (fst (fst s2))) (rolling_hash_list h2 l2) (combine (h2:: rolling_hash_list h2 l2) l2) ->
+  exists s2' t,
+  exec (CryptoDiskLang) u o s2 
+  (hash_all h2 l2)
+       (Finished s2' t).
+  Proof.
+    induction l1; destruct l2; simpl in *; try lia;
+    intros; repeat invert_exec_no_match.
+    do 2 eexists; repeat econstructor.
+    simpl in *.
+    edestruct IHl1.
+    eauto.
+    3:{
+      simpl in *; logic_clean.
+      do 2 eexists; repeat econstructor; eauto.
+      rewrite cons_app.
+      repeat (econstructor; eauto).
+    }
+    eauto.
+    simpl; eauto.
+  Qed.
+
+  Lemma BatchOperations_TS_read_consecutive:
+  forall u n s1 s2 o s1' t h1 h2,
+  exec (CryptoDiskLang) u o s1 
+  (read_consecutive h1 n)
+       (Finished s1' t) ->
+       h2 + n < disk_size ->
+  exists s2' t,
+  exec (CryptoDiskLang) u o s2 
+  (read_consecutive h2 n)
+       (Finished s2' t).
+  Proof.
+    induction n; simpl in *; try lia;
+    intros; repeat invert_exec_no_match.
+    do 2 eexists; repeat econstructor.
+    simpl in *.
+    edestruct IHn.
+    eauto.
+    2:{
+      simpl in *; logic_clean.
+      do 2 eexists; repeat econstructor; eauto.
+      rewrite cons_app.
+      repeat (econstructor; eauto).
+      lia.
+    }
+    lia.
+  Qed.
+
+
+  Lemma BatchOperations_TS_decrypt_all:
+forall u l1 l2 k1 k2 s1 s2 o s1' t,
+
+exec (CryptoDiskLang) u o s1 
+(decrypt_all k1 l1)
+     (Finished s1' t) ->
+
+length l1 = length l2 ->
+
+consistent_with_upds (snd (fst s2)) l2 (map (fun ev => (k2, decrypt k2 ev)) l2) ->
+
+exists s2' t,
+exec (CryptoDiskLang) u o s2 (decrypt_all k2 l2) (Finished s2' t).
+Proof.
+     induction l1; 
+     destruct l2; simpl; intros; 
+     try lia;repeat invert_exec.
+     repeat econstructor.
+     eapply IHl1 in H; cleanup.
+     do 2 eexists; econstructor; eauto.
+     do 3 econstructor; eauto.
+     repeat econstructor; eauto.
+     all: simpl; eauto.
+Qed.
+
+
+(*************************** Crashed TS ********************)
+
+Lemma BatchOperations_TS_hash_all_crashed:
+forall u l1 l2 s1 s2 o s1' h1 h2,
+exec (CryptoDiskLang) u o s1 
+(hash_all h1 l1) (Crashed s1') ->
+length l1 = length l2 ->
+consistent_with_upds (snd (fst (fst s2))) (rolling_hash_list h2 l2) (combine (h2:: rolling_hash_list h2 l2) l2) ->
+exists s2',
+exec (CryptoDiskLang) u o s2 
+(hash_all h2 l2) (Crashed s2').
+Proof.
+  induction l1; destruct l2; simpl in *; try lia;
+  intros; repeat invert_exec_no_match.
+  eexists; repeat econstructor.
+
+  simpl in *; split_ors; cleanup_no_match.
+  repeat invert_exec.
+  eexists; repeat econstructor.
+  repeat invert_exec_no_match.
+  simpl in *; split_ors; cleanup_no_match.
+  edestruct IHl1.
+  eauto.
+  3:{
+    eexists; rewrite cons_app.
+    repeat (econstructor; eauto).
+  }
+  eauto.
+  simpl; eauto.
+
+  repeat invert_exec_no_match.
+  eapply BatchOperations_TS_hash_all in H3; cleanup_no_match.
+  eexists; rewrite cons_app.
+repeat (econstructor; eauto).
+eauto.
+simpl; eauto.
+Qed.
+
+Lemma BatchOperations_TS_read_consecutive_crashed:
+forall u n s1 s2 o s1' h1 h2,
+exec (CryptoDiskLang) u o s1 
+(read_consecutive h1 n)
+     (Crashed s1') ->
+     h2 + n < disk_size ->
+exists s2',
+exec (CryptoDiskLang) u o s2 
+(read_consecutive h2 n) (Crashed s2').
+Proof.
+  induction n; simpl in *; try lia;
+  intros; repeat invert_exec_no_match.
+  eexists; repeat econstructor.
+
+  simpl in *; split_ors; cleanup_no_match.
+  repeat invert_exec.
+  eexists; repeat econstructor.
+  repeat invert_exec_no_match.
+  simpl in *; split_ors; cleanup_no_match.
+
+  edestruct IHn.
+  eauto.
+  2:{
+    eexists; rewrite cons_app.
+    repeat (econstructor; eauto).
+    lia.
+  }
+  lia.
+
+
+  repeat invert_exec_no_match.
+  eapply BatchOperations_TS_read_consecutive in H1; cleanup_no_match.
+  eexists; rewrite cons_app.
+repeat (econstructor; eauto).
+all: lia.
+Qed.
+
+
+Lemma BatchOperations_TS_decrypt_all_crashed:
+forall u l1 l2 k1 k2 s1 s2 o s1',
+
+exec (CryptoDiskLang) u o s1 
+(decrypt_all k1 l1)
+   (Crashed s1') ->
+
+length l1 = length l2 ->
+
+consistent_with_upds (snd (fst s2)) l2 (map (fun ev => (k2, decrypt k2 ev)) l2) ->
+
+exists s2',
+exec (CryptoDiskLang) u o s2 (decrypt_all k2 l2) (Crashed s2').
+Proof.
+   induction l1; 
+   destruct l2; simpl; intros; 
+   try lia;repeat invert_exec.
+   repeat econstructor.
+
+   simpl in *; split_ors; cleanup_no_match.
+  repeat invert_exec.
+  eexists; repeat econstructor.
+  repeat invert_exec_no_match.
+  simpl in *; split_ors; cleanup_no_match.
+  edestruct IHl1.
+  eauto.
+  3:{
+    eexists; rewrite cons_app.
+    repeat (econstructor; eauto).
+  }
+  eauto.
+  simpl; eauto.
+
+  repeat invert_exec_no_match.
+  eapply BatchOperations_TS_decrypt_all in H3; cleanup_no_match.
+  eexists; rewrite cons_app.
+repeat (econstructor; eauto).
+eauto.
+simpl; eauto.
+Qed.
